---
title: "first difference poisson regression"
author: "Xiaolin Cao"
output:
  pdf_document: default
  html_document: default
---

```{r setup, include=FALSE}
knitr::opts_chunk$set(echo = TRUE)
```

$$
\begin{aligned}
Y &= B_0 + B_1X_1 + B_2X_2 \\
\\
first\ difference: Y_2-Y_1 \\
\\
if\ first\ differences\ are\ constant,\ Y_2 - Y_1\ describes\ the\ first\ difference\ completely. \\
\\ 
when\ X_1 &= 0, Y_1 = B_0 + B_2X_2 \\
when\ X_1 &= 1, Y_2 = B_0 + B_1 + B_2X_2} \\
\\
Y_2 - Y_1 &= a
&=e^{B_0}e^{B_1}e^{B_2x_2} - e^{B_0}e^{B_2x_2} \\
&=e^{B_0}e^{B_2X_2}(e^{B_1} - 1) \\

\end{aligned}
$$



$$
\begin{aligned}
log(\frac{P(Y)}{1-P(Y)}) &= B_0 + B_1X_1 + B_2X_2 \\
\frac{P(Y)}{1-P(Y)} &=e^{B_0 + B_1X_1 + B_2X_2} \\
when\ X_1 &= 0, Y_1 = e^{B_0+B_2x_2} \\
when\ X_1 &= 1, Y_2=e^{B_0+B_1+B_2x_2} \\
\\
first\ difference: Y_2-Y_1 \\
\\
&=e^{B_0+B_1+B_2x_2} - e^{B_0+B_2x_2} \\
&=e^{B_0}e^{B_1}e^{B_2x_2} - e^{B_0}e^{B_2x_2} \\
&=e^{B_0}e^{B_2X_2}(e^{B_1} - 1) \\

\end{aligned}
$$

Poisson regression assumes Y has poisson distribution. In this case, with $x_1$ changing from 0 to 1, the difference between Y's is dependent on $x_2$ as well even though there is no interaction term in the model.
